Added definition wordarray_put2 shallow embedding

cogent/examples/wa_connect/Manual_AllRefine.thy
@@ -14,6 +14,13 @@ begin
       \<exists>xs. v = VAbstract (VWA xs) \<and> length x = length xs \<and> (\<forall>i < length xs. xs ! i = VPrim (LU32 (x ! i)))"
 end
 
+overloading
+  wordarray_put2' \<equiv> wordarray_put2
+begin
+definition wordarray_put2':
+ "wordarray_put2' (x :: ('a WordArray, 32 word, 'a) WordArrayPutP) \<equiv> (WordArrayPutP.arr\<^sub>f x)[unat (WordArrayPutP.idx\<^sub>f x) := WordArrayPutP.val\<^sub>f x]" 
+end
+thm wordarray_put2'
 
 thm valRel_WordArrayU32
 
@@ -34,6 +41,27 @@ definition \<xi>_0' :: "(char list, atyp, 32 word) uabsfuns"
                             UPtr p r = z2
                     | _ \<Rightarrow> False)
            else False))" 
+
+definition \<xi>m :: "(char list, vatyp) vabsfuns" 
+  where
+  "\<xi>m x y z = (if x = ''wordarray_put2_0'' then
+                (case y of 
+                      VRecord [VAbstract (VWA xs), 
+                            VPrim (LU32 idx), VPrim (LU32 val)] 
+                        \<Rightarrow> VAbstract (VWA (xs[unat idx := VPrim (LU32 val)])) = z
+                    | _ \<Rightarrow> False)
+           else False)" 
+
+
+definition \<xi>p :: "(char list, vatyp) vabsfuns" 
+  where
+  "\<xi>p x y z = (if x = ''wordarray_put2'' then
+                (case y of 
+                      VRecord [VAbstract (VWA xs), 
+                            VPrim (LU32 idx), VPrim (LU32 val)] 
+                        \<Rightarrow> VAbstract (VWA (xs[unat idx := VPrim (LU32 val)])) = z
+                    | _ \<Rightarrow> False)
+           else False)" 
 
 locale WordArray = main_pp_inferred begin
   definition "abs_repr_u a \<equiv> case a of
@@ -100,6 +128,84 @@ sublocale WordArray \<subseteq> Generated_cogent_shallow _ abs_repr_u abs_typing
   done
 
 context WordArray begin
+lemma "\<lbrakk>\<forall>i<length arrv. arrv ! i = VPrim (LU32 (arr ! i)); length (arr :: 32 word WordArray) = length arrv\<rbrakk> \<Longrightarrow>
+val.matches \<Xi> [VRecord [VAbstract (VWA arrv), VPrim (LU32 (idx :: 32 word)), VPrim (LU32 (val :: 32 word))]]
+         [option.Some (prod.fst (prod.snd Generated_TypeProof.wordarray_put2_u32_type))]"
+  apply (clarsimp simp: val.matches_def Generated_TypeProof.wordarray_put2_u32_type_def Generated_TypeProof.abbreviatedType1_def)
+  apply (rule val.v_t_record)
+   apply (rule val.v_t_r_cons1)
+    apply (rule val.v_t_abstract)
+     apply (clarsimp simp: abs_typing_v_def)
+    apply (clarsimp simp: type_wellformed_all_pretty_def)
+   apply (rule val.v_t_r_cons1)
+    apply auto[1]
+   apply (rule val.v_t_r_cons1)
+    apply auto[1]
+   apply (rule val.v_t_r_empty)
+  apply auto
+  done
+lemma "correspondence_init abs_repr_u abs_typing_v abs_typing_u abs_upd_val'"
+  by (simp add: correspondence_init_axioms)
+
+lemma "value_sem.rename_mono_prog abs_typing_v rename \<Xi> \<xi>m \<xi>p"
+  apply (clarsimp simp: rename_def \<Xi>_def \<xi>m_def \<xi>p_def val.rename_mono_prog_def)
+  apply (rule conjI)
+   apply clarsimp
+   apply (case_tac v; clarsimp)
+   apply (case_tac x4; clarsimp)
+   apply (case_tac a; clarsimp)
+   apply (case_tac list; clarsimp)
+    apply (case_tac x5; clarsimp)
+   apply (case_tac x5; clarsimp)
+   apply (case_tac a; clarsimp)
+   apply (case_tac x1a; clarsimp)
+   apply (case_tac lista; clarsimp)
+   apply (case_tac list; clarsimp)
+    apply (case_tac a; clarsimp)
+    apply (case_tac x1a; clarsimp)
+   apply (case_tac a; clarsimp)
+   apply (case_tac x1a; clarsimp)
+  apply (case_tac ts; clarsimp)
+  apply (case_tac list; clarsimp)
+  apply (case_tac a; clarsimp)
+  apply (case_tac x5; clarsimp)
+  apply (case_tac x1; clarsimp)
+  apply (case_tac "f = ''wordarray_put2''"; clarsimp)
+  done
+
+lemma "val.proc_env_matches \<xi>m \<Xi>"
+  apply (clarsimp simp: val.proc_env_matches_def \<Xi>_def)
+  apply (case_tac "f = ''wordarray_put2_0''")
+   defer
+   apply (case_tac "f = ''wordarray_put2_u32''")
+    apply (clarsimp simp: \<xi>m_def)
+   apply (rule FalseE)
+   apply (clarsimp simp: \<xi>m_def)
+  apply (clarsimp simp: wordarray_put2_0_type_def abbreviatedType1_def \<xi>m_def)
+  apply (case_tac v; clarsimp)
+  apply (case_tac x4; clarsimp)
+  apply (case_tac a; clarsimp)
+  apply (case_tac x5; clarsimp)
+  apply (case_tac list; clarsimp)
+  apply (case_tac a; clarsimp)
+  apply (case_tac x1a; clarsimp)
+  apply (case_tac lista; clarsimp)
+  apply (case_tac a; clarsimp)
+  apply (case_tac x1a; clarsimp)
+  apply (case_tac list; clarsimp)
+  apply (erule val.v_t_recordE)
+  apply (erule val.v_t_r_consE; clarsimp)
+  apply (rule val.v_t_abstract)
+   apply (erule val.v_t_abstractE)
+   apply (clarsimp simp: abs_typing_v_def)
+   apply (erule_tac x = i in allE; clarsimp)
+   apply (case_tac "i = unat x4")
+    apply (rule_tac x = x4a in exI; simp)
+   apply (rule_tac x = x in exI; simp)
+  apply simp
+  done
+
+(*
 theorem manual_generated_theorem:
 "\<lbrakk>Generated_cogent_shallow abs_repr_u abs_typing_v abs_typing_u abs_upd_val';
  \<And>i \<gamma> v' \<Gamma>' \<sigma> st.
@@ -114,15 +220,92 @@ theorem manual_generated_theorem:
            ([], TUnit, TUnit))
          \<Gamma>' \<sigma> st;
  correspondence_init abs_repr_u abs_typing_v abs_typing_u abs_upd_val';
- value_sem.rename_mono_prog abs_typing_v rename \<Xi> \<xi>\<^sub>m \<xi>\<^sub>p; vv\<^sub>m = value_sem.rename_val rename (value_sem.monoval vv\<^sub>p);
- correspondence_init.val_rel_shallow_C abs_repr_u abs_upd_val' rename vv\<^sub>s uv\<^sub>C vv\<^sub>p uv\<^sub>m \<xi>\<^sub>p \<sigma> \<Xi>; proc_ctx_wellformed \<Xi>;
- value_sem.proc_env_matches abs_typing_v \<xi>\<^sub>m \<Xi>;
+ value_sem.rename_mono_prog abs_typing_v rename \<Xi> \<xi>m \<xi>p; vv\<^sub>m = value_sem.rename_val rename (value_sem.monoval vv\<^sub>p);
+ correspondence_init.val_rel_shallow_C abs_repr_u abs_upd_val' rename vv\<^sub>s uv\<^sub>C vv\<^sub>p uv\<^sub>m \<xi>p \<sigma> \<Xi>; proc_ctx_wellformed \<Xi>;
+ value_sem.proc_env_matches abs_typing_v \<xi>m \<Xi>;
  value_sem.matches abs_typing_v \<Xi> [vv\<^sub>m] [option.Some (prod.fst (prod.snd Generated_TypeProof.wordarray_put2_u32_type))]\<rbrakk>
 \<Longrightarrow> correspondence_init.corres_shallow_C abs_repr_u abs_typing_u abs_upd_val' rename (Generated.state_rel abs_repr_u)
-     (Generated_Shallow_Desugar.wordarray_put2_u32 vv\<^sub>s) Generated_TypeProof.wordarray_put2_u32 (wordarray_put2_u32' uv\<^sub>C) \<xi>_0' \<xi>\<^sub>m \<xi>\<^sub>p
+     (Generated_Shallow_Desugar.wordarray_put2_u32 vv\<^sub>s) Generated_TypeProof.wordarray_put2_u32 (wordarray_put2_u32' uv\<^sub>C) \<xi>_0' \<xi>m \<xi>p
      [uv\<^sub>m] [vv\<^sub>m] \<Xi> [option.Some (prod.fst (prod.snd Generated_TypeProof.wordarray_put2_u32_type))] \<sigma> s"
   apply clarsimp
+  apply (subgoal_tac "\<exists>arr idx val. vv\<^sub>s = \<lparr>WordArrayPutP.arr\<^sub>f = arr, idx\<^sub>f = idx, val\<^sub>f = val\<rparr>")
+   prefer 2
+   apply (case_tac vv\<^sub>s; clarsimp)
+  apply clarsimp
+  apply (subgoal_tac "\<exists>arrv. vv\<^sub>p = VRecord [VAbstract (VWA arrv), VPrim (LU32 idx), VPrim (LU32 val)]")
+   prefer 2
+   apply (clarsimp simp: val_rel_shallow_C_def valRel_WordArrayPutP valRel_WordArrayU32)
+  apply clarsimp
+  apply (subgoal_tac "(\<forall>i < length arrv. arrv ! i = VPrim (LU32 (arr ! i))) \<and> length arr = length arrv")
+   prefer 2
+   apply (clarsimp simp: val_rel_shallow_C_def valRel_WordArrayPutP valRel_WordArrayU32)
+  apply clarsimp
+  apply (subgoal_tac "val_rel uv\<^sub>m uv\<^sub>C")
+  prefer 2
+   apply (clarsimp simp: val_rel_shallow_C_def)
+  apply (clarsimp simp: val_rel_simp)
+  apply (rule_tac vv\<^sub>s = vv\<^sub>s and 
+                  vv\<^sub>p = vv\<^sub>p and
+                   \<tau>o = "prod.snd (prod.snd Generated_TypeProof.wordarray_put2_u32_type)" and 
+                  prog\<^sub>p = "expr.Let (Var 0) (App (AFun ''wordarray_put2'' [TPrim (Num U32)]) (Var 0))"
+                      in corres_shallow_C_intro)
+          apply (clarsimp simp: Generated_TypeProof.wordarray_put2_u32_def rename_def)
+         apply simp
+        apply simp
+       apply simp
+  
+       apply (clarsimp simp: Generated_TypeProof.wordarray_put2_u32_type_def
+                             Generated_TypeProof.abbreviatedType1_def
+                             Generated_TypeProof.wordarray_put2_u32_def)
+(*
+       apply (rule_tac ?\<Gamma>1.0 = "[option.Some (TRecord 
+                                    [(''arr'', TCon ''WordArray'' [TPrim (Num U32)] (Boxed Writable undefined), Present),
+                                     (''idx'', TPrim (Num U32), Present), 
+                                     (''val'', TPrim (Num U32), Present)]  Unboxed)]" and 
+                       ?\<Gamma>2.0 = "[]" and 
+                       t = "TCon ''WordArray'' [TPrim (Num U32)] (Boxed Writable undefined)" in typing_let)
+         
+*)
+       defer
+      apply (clarsimp simp: Generated_TypeProof.wordarray_put2_u32_def)
+      apply (monad_eq simp: wordarray_put2_u32'_def)
+(*
+       apply (rule_tac ?\<Gamma>1.0 = "[option.Some (prod.fst (prod.snd Generated_TypeProof.wordarray_put2_u32_type))]" and
+                       ?\<Gamma>2.0 = "[]" and
+                       t = "(prod.fst (prod.snd Generated_TypeProof.wordarray_put2_u32_type))" in corres_let)
+  *)
+      defer
+      defer
+      apply simp
+     apply (clarsimp simp: val_rel_shallow_C_def)
+    prefer 3
+    apply (clarsimp simp: val.scorres_def)
+    apply (erule v_sem_varE; clarsimp)
+    apply (erule v_sem_appE)
+     prefer 2
+     apply (rule FalseE)
+     apply blast
+    apply (erule v_sem_afunE)
+    apply (erule v_sem_varE)
+    apply (clarsimp simp: \<xi>p_def)
+    apply (clarsimp simp: Generated_Shallow_Desugar.wordarray_put2_u32_def wordarray_put2' valRel_WordArrayU32)
+    apply (erule_tac x = i in allE; clarsimp)
+    apply (case_tac "i = unat idx"; clarsimp)
+
+      apply (rule_tac ?\<Gamma>1.0 = "[option.Some (prod.fst (prod.snd Generated_TypeProof.wordarray_put2_u32_type))]" and
+                       ?\<Gamma>2.0 = "[]" and
+                       t = "(prod.fst (prod.snd Generated_TypeProof.wordarray_put2_u32_type))" in typing_let)
+     prefer 2
+     apply (rule typing_var; clarsimp simp: Cogent.empty_def)
+     apply (clarsimp simp: weakening_conv_all_nth)
+     apply (rule keep)
+     apply (clarsimp simp: Generated_TypeProof.wordarray_put2_u32_type_def abbreviatedType1_def)
+    apply (clarsimp simp: Generated_TypeProof.wordarray_put2_u32_type_def abbreviatedType1_def)
+    apply (clarsimp simp: split_conv_all_nth)
+
+(*  apply (clarsimp simp: corres_shallow_C_def)*)
   oops
+*)
 (*
 \<xi>_m == monomorphic value semantics contexts for values
 \<xi>_p == polymorphic ...
@@ -132,5 +315,115 @@ vv_m == value of the argument of the function, i.e. wordarray_put2, in the monom
 uv_m == value of the argument of the function, i.e. wordarray_put2, in the monomorphic update semantics
 uv_c == value of the argument of the function, i.e. wordarray_put2, in the autocorres generated C
 *)
+
+
+theorem manual_generated_theorem':
+"\<lbrakk>Generated_cogent_shallow abs_repr_u abs_typing_v abs_typing_u abs_upd_val';
+ \<And>i \<gamma> v' \<Gamma>' \<sigma> st.
+    \<lbrakk>i < length \<gamma>; val_rel (\<gamma> ! i) v'; \<Gamma>' ! i = option.Some (prod.fst (prod.snd wordarray_put2_0_type))\<rbrakk>
+    \<Longrightarrow> update_sem_init.corres abs_typing_u abs_repr_u (Generated.state_rel abs_repr_u) (App (AFun ''wordarray_put2_0'' []) (Var i))
+         (do x <- wordarray_put2_0' v';
+             gets (\<lambda>s. x)
+          od)
+         \<xi>_0' \<gamma>
+         (assoc_lookup
+           [(''wordarray_put2_0'', wordarray_put2_0_type), (''wordarray_put2_u32'', Generated_TypeProof.wordarray_put2_u32_type)]
+           ([], TUnit, TUnit))
+         \<Gamma>' \<sigma> st;
+ correspondence_init abs_repr_u abs_typing_v abs_typing_u abs_upd_val';
+ value_sem.rename_mono_prog abs_typing_v rename \<Xi> \<xi>m \<xi>p; vv\<^sub>m = value_sem.rename_val rename (value_sem.monoval vv\<^sub>p);
+ correspondence_init.val_rel_shallow_C abs_repr_u abs_upd_val' rename vv\<^sub>s uv\<^sub>C vv\<^sub>p uv\<^sub>m \<xi>p \<sigma> \<Xi>; proc_ctx_wellformed \<Xi>;
+ value_sem.proc_env_matches abs_typing_v \<xi>m \<Xi>;
+ value_sem.matches abs_typing_v \<Xi> [vv\<^sub>m] [option.Some (prod.fst (prod.snd Generated_TypeProof.wordarray_put2_u32_type))]\<rbrakk>
+\<Longrightarrow> correspondence_init.corres_shallow_C abs_repr_u abs_typing_u abs_upd_val' rename (Generated.state_rel abs_repr_u)
+     (Generated_Shallow_Desugar.wordarray_put2_u32 vv\<^sub>s) Generated_TypeProof.wordarray_put2_u32 (wordarray_put2_u32' uv\<^sub>C) \<xi>_0' \<xi>m \<xi>p
+     [uv\<^sub>m] [vv\<^sub>m] \<Xi> [option.Some (prod.fst (prod.snd Generated_TypeProof.wordarray_put2_u32_type))] \<sigma> s"
+  apply clarsimp
+  apply (subgoal_tac "\<exists>arr idx val. vv\<^sub>s = \<lparr>WordArrayPutP.arr\<^sub>f = arr, idx\<^sub>f = idx, val\<^sub>f = val\<rparr>")
+   prefer 2
+   apply (case_tac vv\<^sub>s; clarsimp)
+  apply clarsimp
+  apply (subgoal_tac "\<exists>arrv. vv\<^sub>p = VRecord [VAbstract (VWA arrv), VPrim (LU32 idx), VPrim (LU32 val)]")
+   prefer 2
+   apply (clarsimp simp: val_rel_shallow_C_def valRel_WordArrayPutP valRel_WordArrayU32)
+  apply clarsimp
+  apply (subgoal_tac "(\<forall>i < length arrv. arrv ! i = VPrim (LU32 (arr ! i))) \<and> length arr = length arrv")
+   prefer 2
+   apply (clarsimp simp: val_rel_shallow_C_def valRel_WordArrayPutP valRel_WordArrayU32)
+  apply clarsimp
+  apply (subgoal_tac "val_rel uv\<^sub>m uv\<^sub>C")
+  prefer 2
+   apply (clarsimp simp: val_rel_shallow_C_def)
+  apply (clarsimp simp: val_rel_simp)
+  apply (drule_tac x = 0 in meta_spec)
+  apply (drule_tac x = "[URecord [(UPtr (ptr_val (arr_C uv\<^sub>C)) repr, b), (UPrim (LU32 (idx_C uv\<^sub>C)), ba),
+                            (UPrim (LU32 (val_C uv\<^sub>C)), bb)]]" in meta_spec)
+  apply (drule_tac x = uv\<^sub>C in meta_spec)
+  apply (drule_tac x = "[option.Some (prod.fst (prod.snd Generated_TypeProof.wordarray_put2_u32_type))]" in meta_spec)
+  apply (drule_tac x = \<sigma> in meta_spec)
+  apply (drule_tac x = s in meta_spec)
+  apply (clarsimp simp:  corres_shallow_C_def)
+  apply (monad_eq simp: wordarray_put2_u32'_def)
+  apply (drule  meta_mp)
+   apply (clarsimp simp: Generated_TypeProof.wordarray_put2_u32_type_def 
+                         Generated_TypeProof.abbreviatedType1_def 
+                         wordarray_put2_0_type_def)
+  apply (clarsimp simp: corres_def)
+  apply (erule impE)
+   apply (clarsimp simp: \<Xi>_def)
+  apply (erule impE)
+   apply (clarsimp simp: \<Xi>_def)
+  apply (erule impE)
+   apply (rule_tac x = r in exI)
+   apply (rule_tac x = x in exI)
+   apply (frule u_v_matches_to_matches_ptrs)
+   apply (clarsimp simp: \<Xi>_def
+                         Generated_TypeProof.wordarray_put2_u32_type_def 
+                         Generated_TypeProof.abbreviatedType1_def 
+                         wordarray_put2_0_type_def)
+  apply clarsimp
+  apply (erule_tac x = r' in allE)
+  apply (erule_tac x = s' in allE)
+  apply clarsimp
+  apply (rule_tac x = \<sigma>' in exI)
+  apply (rule_tac x = ra in exI)
+  apply (clarsimp simp: Generated_TypeProof.wordarray_put2_u32_def)
+  apply (rule conjI)
+   apply (rule_tac \<sigma>' = \<sigma> and a' = uv\<^sub>m in u_sem_let)
+  apply clarsimp
+    apply (rule u_sem_var[where i = 0 and \<gamma> = "[_]", simplified])
+   apply clarsimp
+   apply (rule u_sem_abs_app)
+     apply (rule u_sem_afun)
+    apply (rule u_sem_var)
+   apply (erule u_sem_appE; clarsimp)
+    apply (erule u_sem_afunE; clarsimp)
+    apply (erule u_sem_varE; clarsimp)
+   apply (erule u_sem_afunE; clarsimp)
+  apply (rule_tac x = "VAbstract (VWA (arrv[unat idx := VPrim (LU32 val)]))" in exI)
+  apply clarsimp
+  apply (rule conjI)
+   apply (rule v_sem_let)
+    apply (rule v_sem_var)
+   apply (rule v_sem_abs_app)
+     apply (rule v_sem_afun)
+    apply (rule v_sem_var)
+   apply (clarsimp simp: \<xi>m_def)
+  apply (clarsimp simp: Generated_Shallow_Desugar.wordarray_put2_u32_def wordarray_put2')
+  apply (clarsimp simp: val_rel_shallow_C_def)
+  apply (clarsimp simp: valRel_WordArrayU32)
+  apply (rule conjI)
+   apply clarsimp
+   apply (erule_tac x = i in allE)
+   apply clarsimp
+   apply (case_tac "i = unat idx"; clarsimp)
+  apply (rule_tac x = "TCon ''WordArray'' [TPrim (Num U32)] (Boxed Writable undefined)" in exI)
+  apply (rule_tac x = rb in exI)
+  apply (rule_tac x = xa in exI)
+  apply (clarsimp simp: val_rel_simp)
+  thm u_v_p_abs_w
+  apply (rule  u_v_p_abs_w)   
+  sorry
+
 end (* of context *)
 end
