cogent/isa/UpdateSemantics.thy
@@ -157,7 +157,6 @@ where
                      ; \<xi> , \<gamma> \<turnstile>* (\<sigma>', xs) \<Down>! (\<sigma>'', vs)
                      \<rbrakk> \<Longrightarrow>  \<xi> , \<gamma> \<turnstile>* (\<sigma>, x # xs) \<Down>! (\<sigma>'', v # vs)"
 
-
 definition frame :: "('f, 'a, 'l) store \<Rightarrow> 'l set \<Rightarrow> ('f, 'a, 'l) store \<Rightarrow> 'l set \<Rightarrow> bool"
            where
   "frame \<sigma> pi \<sigma>' po \<equiv> \<forall>p. (p \<in> pi \<and> p \<notin> po \<longrightarrow> \<sigma>' p = None)
