cogent/isa/ValueSemantics.thy
@@ -225,6 +225,7 @@ inductive_cases v_t_primE     [elim]: "\<Xi> \<turnstile> VPrim l :v TPrim (Num 
 
 inductive_cases v_t_r_emptyE  [elim]: "\<Xi> \<turnstile>* [] :vr \<tau>s"
 inductive_cases v_t_r_consE   [elim]: "\<Xi> \<turnstile>* (x # xs) :vr \<tau>s"
+inductive_cases v_t_abstractE [elim]: "\<Xi> \<turnstile> VAbstract a :v TCon n ts s"
 
 
 definition vval_typing_all :: "('f \<Rightarrow> poly_type) \<Rightarrow> ('f, 'a) vval list \<Rightarrow> type list \<Rightarrow> bool"
